dataplane/Examples/Batch/Batch_Op_Nop_Invariant.thy
@@ -5,10 +5,10 @@ imports
   "../../Timely/Tree_Nop_Invariant"
 begin
 
-section ‹The Optimized and Plain Compiled Batch Programs are Equivalent›
+section \<open>The Optimized and Plain Compiled Batch Programs are Equivalent\<close>
 
-text ‹Both leaves are @{const builder_op} instances, so
-@{thm [source] compile_dataflow_opt_wbisim_generic} applies.›
+text \<open>Both leaves are @{const builder_op} instances, so
+@{thm [source] compile_dataflow_opt_wbisim_generic} applies.\<close>
 
 lemma builder_tree_G_dt:
   "builder_tree (G_dt f ips bt)"
@@ -19,11 +19,11 @@ lemma distinct_tree_ids_G_dt:
   by simp
 
 theorem compiled_batch_op_opt_wbisim:
-  "compile_dataflow_opt (λ _. []) (batch_tree ins f) ≈ compiled_batch_op ins f"
+  "compile_dataflow_opt (\<lambda> _. []) (batch_tree ins f) \<approx> compiled_batch_op ins f"
   by (rule compile_dataflow_opt_wbisim_generic[OF builder_tree_G_dt distinct_tree_ids_G_dt])
 
 theorem compiled_batch_op_opt_wtraces:
-  "compile_dataflow_opt (λ _. []) (batch_tree ins f) ≡⇩t compiled_batch_op ins f"
+  "compile_dataflow_opt (\<lambda> _. []) (batch_tree ins f) \<equiv>\<^sub>t compiled_batch_op ins f"
   by (rule wbisim_wtraces[OF compiled_batch_op_opt_wbisim])
 
 end
