dataplane/Examples/Weakly_Connected_Components/Label_Propagation_Nop_Invariant.thy
@@ -5,7 +5,7 @@ imports
   "../../Timely/Tree_Nop_Invariant"
 begin
 
-section ‹The Optimized and Plain Compiled Label Propagation Programs are Equivalent›
+section \<open>The Optimized and Plain Compiled Label Propagation Programs are Equivalent\<close>
 
 lemma builder_tree_G:
   "builder_tree (G_dt inp_state label_state incr_state)"
@@ -17,13 +17,13 @@ lemma distinct_tree_ids_G:
   by simp
 
 theorem compiled_label_propagation_wbisim:
-  "compiled inp ≈ compile_dataflow (λ _. [])
+  "compiled inp \<approx> compile_dataflow (\<lambda> _. [])
      (G_dt (initial_state_input inp) initial_state_label_prop
         (initial_state_increment (MyPair 0 1)))"
   by (rule compile_dataflow_opt_wbisim_generic[OF builder_tree_G distinct_tree_ids_G])
 
 theorem compiled_label_propagation_wtraces:
-  "compiled inp ≡⇩t compile_dataflow (λ _. [])
+  "compiled inp \<equiv>\<^sub>t compile_dataflow (\<lambda> _. [])
      (G_dt (initial_state_input inp) initial_state_label_prop
         (initial_state_increment (MyPair 0 1)))"
   by (rule wbisim_wtraces[OF compiled_label_propagation_wbisim])
