dataplane/Examples/Weakly_Connected_Components/Label_Propagation_Op_Tests.thy
@@ -4,12 +4,12 @@ imports
   Label_Propagation_Nop_Invariant
 begin
 
-section ‹Executable Tests for the Label Propagation Program›
+section \<open>Executable Tests for the Label Propagation Program\<close>
 
-text ‹The tests compare @{const lset} of the trace, not the trace itself: the
-  order in which the outputs come out is an artifact of the schedule.›
+text \<open>The tests compare @{const lset} of the trace, not the trace itself: the
+  order in which the outputs come out is an artifact of the schedule.\<close>
 
-abbreviation ‹test_input1 ≡ llist_of [Mint (MyPair 1 0), Mint (MyPair 2 0), Data ⊥ (0, 1), Data (MyPair 1 0) (3, 4), Data ⊥ (1, 2), Data (MyPair 2 0) (4, 5)]›
+abbreviation \<open>test_input1 \<equiv> llist_of [Mint (MyPair 1 0), Mint (MyPair 2 0), Data \<bottom> (0, 1), Data (MyPair 1 0) (3, 4), Data \<bottom> (1, 2), Data (MyPair 2 0) (4, 5)]\<close>
 
 value "list_connections (dataflow_tree_to_graph (G_dt (initial_state_input test_input1) initial_state_label_prop (initial_state_increment (MyPair 0 1))))"
 
@@ -18,69 +18,69 @@ value [GHC] "unit_test (lset (lmap show_Outs (trace_exec (compiled test_input1))
   (Loc 1 (Src 0), Inr {{3, 4}, {1, 2, 0, 1}}, MyPair 1 0),
   (Loc 1 (Src 0), Inr {{4, 5, 3, 4}, {1, 2, 0, 1}}, MyPair 2 0)])"
 
-abbreviation ‹test_input2 ≡ llist_of [Mint (MyPair 1 0), Mint (MyPair 2 0), Data ⊥ (1, 2), Data ⊥ (0, 1), Data (MyPair 1 0) (3, 4), Data (MyPair 2 0) (4, 5), Mint (MyPair 3 0), Data (MyPair 3 0) (2, 3)]›
-value [GHC] ‹unit_test (lset (lmap show_Outs (trace_exec (compiled test_input2))))
+abbreviation \<open>test_input2 \<equiv> llist_of [Mint (MyPair 1 0), Mint (MyPair 2 0), Data \<bottom> (1, 2), Data \<bottom> (0, 1), Data (MyPair 1 0) (3, 4), Data (MyPair 2 0) (4, 5), Mint (MyPair 3 0), Data (MyPair 3 0) (2, 3)]\<close>
+value [GHC] \<open>unit_test (lset (lmap show_Outs (trace_exec (compiled test_input2))))
  (set [(Loc 1 (Src 0), Inr {{1, 1, 0, 2}}, MyPair 0 0),
   (Loc 1 (Src 0), Inr {{3, 4}, {1, 1, 0, 2}}, MyPair 1 0),
   (Loc 1 (Src 0), Inr {{4, 5, 3, 4}, {1, 1, 0, 2}}, MyPair 2 0),
   (Loc 1 (Src 0),
    Inr {{4, 5, 3, 4, 2, 1, 3, 1, 0, 2}},
-   MyPair 3 0)])›
+   MyPair 3 0)])\<close>
 
-abbreviation ‹test_input3 ≡
-  llist_of [Mint (MyPair 1 0), Mint (MyPair 2 0), Data ⊥ (0, 1), Data (MyPair 1 0) (2, 3),
-  Mint (MyPair 3 0), Data (MyPair 3 0) (1, 2), Mint (MyPair 4 0), Data (MyPair 4 0) (4, 5), Mint (MyPair 5 0), Data (MyPair 5 0) (3, 5)]›
-value [GHC] ‹unit_test (lset (lmap show_Outs (trace_exec (compiled test_input3))))
+abbreviation \<open>test_input3 \<equiv>
+  llist_of [Mint (MyPair 1 0), Mint (MyPair 2 0), Data \<bottom> (0, 1), Data (MyPair 1 0) (2, 3),
+  Mint (MyPair 3 0), Data (MyPair 3 0) (1, 2), Mint (MyPair 4 0), Data (MyPair 4 0) (4, 5), Mint (MyPair 5 0), Data (MyPair 5 0) (3, 5)]\<close>
+value [GHC] \<open>unit_test (lset (lmap show_Outs (trace_exec (compiled test_input3))))
  (set [(Loc 1 (Src 0), Inr {{0, 1}, {0, 1}}, MyPair 0 0),
   (Loc 1 (Src 0), Inr { {2, 1, 3, 1, 0, 2}}, MyPair 3 0),
   (Loc 1 (Src 0), Inr {{2, 1, 3, 1, 0, 2}, {4, 5}}, MyPair 4 0),
   (Loc 1 (Src 0), Inr {{2, 3}, {2, 3}, {0, 1}}, MyPair 1 0),
   (Loc 1 (Src 0),
    Inr {{5, 2, 1, 3, 4, 0}},
-   MyPair 5 0)])›
+   MyPair 5 0)])\<close>
 
-abbreviation ‹test_input4 ≡
+abbreviation \<open>test_input4 \<equiv>
   llist_of [Mint (MyPair 1 0), Mint (MyPair 2 0),Mint (MyPair 3 0),Mint (MyPair 4 0), Mint (MyPair 5 0),
-   Data (MyPair 5 0) (3, 5), Data (MyPair 4 0) (4, 5), Data (MyPair 3 0) (1, 2), Data (MyPair 1 0) (2, 3), Data ⊥ (0, 1)]›
-value [GHC] ‹unit_test (lset (lmap show_Outs (trace_exec (compiled test_input4))))
+   Data (MyPair 5 0) (3, 5), Data (MyPair 4 0) (4, 5), Data (MyPair 3 0) (1, 2), Data (MyPair 1 0) (2, 3), Data \<bottom> (0, 1)]\<close>
+value [GHC] \<open>unit_test (lset (lmap show_Outs (trace_exec (compiled test_input4))))
  (set [(Loc 1 (Src 0), Inr {{0, 1}, {0, 1}}, MyPair 0 0),
   (Loc 1 (Src 0), Inr { {2, 1, 3, 1, 0, 2}}, MyPair 3 0),
   (Loc 1 (Src 0), Inr {{2, 1, 3, 1, 0, 2}, {4, 5}}, MyPair 4 0),
   (Loc 1 (Src 0), Inr {{2, 3}, {2, 3}, {0, 1}}, MyPair 1 0),
   (Loc 1 (Src 0),
    Inr {{5, 2, 1, 3, 4, 0}},
-   MyPair 5 0)])›
+   MyPair 5 0)])\<close>
 
-abbreviation ‹test_input5 ≡
-  llist_of [Mint (MyPair 1 0), Mint (MyPair 2 0), Data ⊥ (0, 1), Drop ⊥, Data (MyPair 1 0) (2, 3), Drop (MyPair 1 0),
-  Mint (MyPair 3 0), Drop (MyPair 2 0), Data (MyPair 3 0) (1, 2), Mint (MyPair 4 0), Drop (MyPair 3 0), Data (MyPair 4 0) (4, 5), Mint (MyPair 5 0),  Drop (MyPair 4 0), Data (MyPair 5 0) (3, 5)]›
-value [GHC] ‹unit_test (lset (lmap show_Outs (trace_exec (compiled test_input5))))
+abbreviation \<open>test_input5 \<equiv>
+  llist_of [Mint (MyPair 1 0), Mint (MyPair 2 0), Data \<bottom> (0, 1), Drop \<bottom>, Data (MyPair 1 0) (2, 3), Drop (MyPair 1 0),
+  Mint (MyPair 3 0), Drop (MyPair 2 0), Data (MyPair 3 0) (1, 2), Mint (MyPair 4 0), Drop (MyPair 3 0), Data (MyPair 4 0) (4, 5), Mint (MyPair 5 0),  Drop (MyPair 4 0), Data (MyPair 5 0) (3, 5)]\<close>
+value [GHC] \<open>unit_test (lset (lmap show_Outs (trace_exec (compiled test_input5))))
  (set [(Loc 1 (Src 0), Inr {{0, 1}, {0, 1}}, MyPair 0 0),
   (Loc 1 (Src 0), Inr { {2, 1, 3, 1, 0, 2}}, MyPair 3 0),
   (Loc 1 (Src 0), Inr {{2, 1, 3, 1, 0, 2}, {4, 5}}, MyPair 4 0),
   (Loc 1 (Src 0), Inr {{2, 3}, {2, 3}, {0, 1}}, MyPair 1 0),
   (Loc 1 (Src 0),
    Inr {{5, 2, 1, 3, 4, 0}},
-   MyPair 5 0)])›
+   MyPair 5 0)])\<close>
 
-abbreviation ‹test_input6 ≡
+abbreviation \<open>test_input6 \<equiv>
   llist_of [Mint (MyPair 1 0), Mint (MyPair 4 0), Mint (MyPair 3 0),
    Data (MyPair 3 0) (1, 2), Data (MyPair 4 0) (4, 5), Mint (MyPair 2 0),
-   Data ⊥ (0, 1), Data (MyPair 1 0) (2, 3), Mint (MyPair 5 0), Data (MyPair 5 0) (3, 5)]›
-value [GHC] ‹unit_test (lset (lmap show_Outs (trace_exec (compiled test_input6))))
+   Data \<bottom> (0, 1), Data (MyPair 1 0) (2, 3), Mint (MyPair 5 0), Data (MyPair 5 0) (3, 5)]\<close>
+value [GHC] \<open>unit_test (lset (lmap show_Outs (trace_exec (compiled test_input6))))
  (set [(Loc 1 (Src 0), Inr {{0, 1}, {0, 1}}, MyPair 0 0),
   (Loc 1 (Src 0), Inr { {2, 1, 3, 1, 0, 2}}, MyPair 3 0),
   (Loc 1 (Src 0), Inr {{2, 1, 3, 1, 0, 2}, {4, 5}}, MyPair 4 0),
   (Loc 1 (Src 0), Inr {{2, 3}, {2, 3}, {0, 1}}, MyPair 1 0),
   (Loc 1 (Src 0),
    Inr {{5, 2, 1, 3, 4, 0}},
-   MyPair 5 0)])›
+   MyPair 5 0)])\<close>
 
-abbreviation ‹test_input7 ≡
-  llist_of [ Data ⊥ (0, 6), Mint (MyPair 1 0), Mint (MyPair 4 0), Mint (MyPair 3 0),
+abbreviation \<open>test_input7 \<equiv>
+  llist_of [ Data \<bottom> (0, 6), Mint (MyPair 1 0), Mint (MyPair 4 0), Mint (MyPair 3 0),
    Data (MyPair 3 0) (1, 2), Data (MyPair 4 0) (4, 5), Mint (MyPair 2 0),
-   Data ⊥ (0, 1), Data (MyPair 1 0) (2, 3), Mint (MyPair 5 0), Data (MyPair 5 0) (3, 5), Data (MyPair 5 0) (6, 5)]›
-value [GHC] ‹unit_test (lset (lmap show_Outs (trace_exec (compiled test_input7))))
+   Data \<bottom> (0, 1), Data (MyPair 1 0) (2, 3), Mint (MyPair 5 0), Data (MyPair 5 0) (3, 5), Data (MyPair 5 0) (6, 5)]\<close>
+value [GHC] \<open>unit_test (lset (lmap show_Outs (trace_exec (compiled test_input7))))
  (set [(Loc 1 (Src 0), Inr {{0, 0, 1, 6}}, MyPair 0 0),
   (Loc 1 (Src 0),
    Inr {{2, 3, 1, 2, 0, 0, 1, 6}},
@@ -91,16 +91,16 @@ value [GHC] ‹unit_test (lset (lmap show_Outs (trace_exec (compiled test_input7
   (Loc 1 (Src 0), Inr {{2, 3}, {0, 0, 1, 6}}, MyPair 1 0),
   (Loc 1 (Src 0),
    Inr {{5, 2, 3, 4, 6, 1, 0}},
-   MyPair 5 0)])›
+   MyPair 5 0)])\<close>
 
-abbreviation ‹test_input8 ≡
-  llist_of [Data ⊥ (0, 6), Mint (MyPair 3 0), Data (MyPair 3 0) (1, 2), Data ⊥ (0, 1)]›
-value [GHC] ‹unit_test (lset (lmap show_Outs (trace_exec (compiled test_input8))))
+abbreviation \<open>test_input8 \<equiv>
+  llist_of [Data \<bottom> (0, 6), Mint (MyPair 3 0), Data (MyPair 3 0) (1, 2), Data \<bottom> (0, 1)]\<close>
+value [GHC] \<open>unit_test (lset (lmap show_Outs (trace_exec (compiled test_input8))))
  (set [(Loc 1 (Src 0), Inr {{0, 1, 6}}, MyPair 0 0),
-  (Loc 1 (Src 0), Inr {{1, 2, 0, 6}}, MyPair 3 0)])›
+  (Loc 1 (Src 0), Inr {{1, 2, 0, 6}}, MyPair 3 0)])\<close>
 
-abbreviation ‹test_input9 ≡
-  llist_of [ Data ⊥ (0, 6), Data ⊥ (0, 1), Data (MyPair 1 0) (2, 3)]›
+abbreviation \<open>test_input9 \<equiv>
+  llist_of [ Data \<bottom> (0, 6), Data \<bottom> (0, 1), Data (MyPair 1 0) (2, 3)]\<close>
 value [GHC] "unit_test (lset (lmap show_Outs (trace_exec (compiled test_input9))))
  (set [(Loc 1 (Src 0), Inr {{0, 1, 6}}, MyPair 0 0), (Loc 1 (Src 0), Inr {{2, 3}, {0, 1, 6}}, MyPair 1 0)])"
 
