dataplane/Lib/DataplaneUtils.thy
@@ -4,27 +4,27 @@ imports
   ZmsetUtils
 begin
 
-abbreviation "isr x ≡ ¬ (isl x)"
+abbreviation "isr x \<equiv> \<not> (isl x)"
 
-section ‹General-Purpose Facts›
+section \<open>General-Purpose Facts\<close>
 
-text ‹Congruence rules, lazy list shifts, and relational sets.›
+text \<open>Congruence rules, lazy list shifts, and relational sets.\<close>
 
 lemma ldropWhile_LConsD:
-  "ldropWhile P lxs = LCons x lxs' ⟹
-   ¬ P x"
+  "ldropWhile P lxs = LCons x lxs' \<Longrightarrow>
+   \<not> P x"
   by (metis lhd_ldropWhile llist.disc(2) llist.sel(1) lnull_ldropWhile)
 
 lemma arg_cong3:
-  "a = b ⟹ c = d ⟹ e = g ⟹ f a c e = f b d g"
+  "a = b \<Longrightarrow> c = d \<Longrightarrow> e = g \<Longrightarrow> f a c e = f b d g"
   by fast
 
 lemma arg_cong4:
-  "a = b ⟹ c = d ⟹ e = g ⟹ h = i ⟹ f a c e h  = f b d g i"
+  "a = b \<Longrightarrow> c = d \<Longrightarrow> e = g \<Longrightarrow> h = i \<Longrightarrow> f a c e h  = f b d g i"
   by fast
 
 lemma arg_cong5:
-  "a = b ⟹ c = d ⟹ e = g ⟹ h = i ⟹ j = k ⟹ f a c e h j  = f b d g i k"
+  "a = b \<Longrightarrow> c = d \<Longrightarrow> e = g \<Longrightarrow> h = i \<Longrightarrow> j = k \<Longrightarrow> f a c e h j  = f b d g i k"
   by fast
 
 lemma lmap_lshift[simp]:
@@ -37,32 +37,32 @@ lemma lfinite_lshift[simp]:
 
 
 lemma rel_set_image:
-  "rel_set R (f ` A) B ⟷ rel_set (λ x. R (f x)) A B"
-  "rel_set S A (g ` B) ⟷ rel_set (λ x y. S x (g y)) A B"
+  "rel_set R (f ` A) B \<longleftrightarrow> rel_set (\<lambda> x. R (f x)) A B"
+  "rel_set S A (g ` B) \<longleftrightarrow> rel_set (\<lambda> x y. S x (g y)) A B"
   unfolding rel_set_def
   apply auto
   done
 
 
-section ‹Buffer Heads and Enqueues›
+section \<open>Buffer Heads and Enqueues\<close>
 
-text ‹How BHD and BENQ interact with appending.›
+text \<open>How BHD and BENQ interact with appending.\<close>
 
 lemma BAPPEND_BENQ_BHD':
-  "buf1 p ≠ [] ⟹ BHD p buf1 = x ⟹ (BTL p buf1) >> (BENQ p x buf2) = buf1 >> buf2"
+  "buf1 p \<noteq> [] \<Longrightarrow> BHD p buf1 = x \<Longrightarrow> (BTL p buf1) >> (BENQ p x buf2) = buf1 >> buf2"
   unfolding BULK_BENQ_def BTL_def BENQ_def BHD_def by force
 
 lemma BHD_map[simp]:
-  "buf p ≠ [] ⟹
-   BHD p (λx. map f (buf x)) = f (BHD p buf)"
+  "buf p \<noteq> [] \<Longrightarrow>
+   BHD p (\<lambda>x. map f (buf x)) = f (BHD p buf)"
   unfolding BHD_def
   apply (auto simp add: hd_map)
   done
 
 
-section ‹Concatenations of Lazy Lists›
+section \<open>Concatenations of Lazy Lists\<close>
 
-text ‹Heads and tails of concatenated, zipped lazy lists.›
+text \<open>Heads and tails of concatenated, zipped lazy lists.\<close>
 
 
 
