dataplane/Timely/Propagation_Idempotence.thy
@@ -4,24 +4,24 @@ imports
   Propagation_Exec
 begin
 
-section ‹Idempotence of propagate_all›
+section \<open>Idempotence of propagate_all\<close>
 
-text ‹If propagate_all terminates, the resulting configuration has an empty worklist.›
+text \<open>If propagate_all terminates, the resulting configuration has an empty worklist.\<close>
 
 lemma propagate_all_empty_worklist:
-  "propagate_all summary conf = Some conf' ⟹ worklist_is_empty summary conf'"
+  "propagate_all summary conf = Some conf' \<Longrightarrow> worklist_is_empty summary conf'"
   unfolding propagate_all_def
   by (drule while_option_stop) simp
 
-text ‹On a quiescent configuration, propagate_all is the identity.›
+text \<open>On a quiescent configuration, propagate_all is the identity.\<close>
 
 lemma propagate_all_quiescent:
-  "worklist_is_empty summary conf ⟹ propagate_all summary conf = Some conf"
+  "worklist_is_empty summary conf \<Longrightarrow> propagate_all summary conf = Some conf"
   unfolding propagate_all_def
   by (subst while_option_unfold) simp
 
 lemma propagate_all_idem:
-  "propagate_all summary conf = Some conf' ⟹ propagate_all summary conf' = Some conf'"
+  "propagate_all summary conf = Some conf' \<Longrightarrow> propagate_all summary conf' = Some conf'"
   by (rule propagate_all_quiescent[OF propagate_all_empty_worklist])
 
 end
